src-lite/transfer/properties.v
@@ -1,0 +1,541 @@
+Require Import transfer.syntax.
+Require Import lc.
+Require Import Program.Equality.
+Require Import list_properties.
+
+Hint Extern 2 (_ = _) => simpl; congruence : core.
+
+Lemma inst_e_det : forall e' Θ e1,
+  uniq Θ → Θ ⊩ e' ⇝ e1 → forall e2, Θ ⊩ e' ⇝ e2 → e1 = e2.
+Proof.
+  intros * Uniq H1.
+  induction H1; intros e2 H2; inversion H2; subst; auto;
+  (* solving all the binds with binds_unique in metalib *)
+  try match goal with
+  | H1 : binds ?x ?e1 ?c , H2 : binds ?x ?e2 ?c |- _ = _ =>
+    let E := fresh "E" in
+      assert (e1 = e2) as E by (eapply binds_unique; eauto);
+      inversion E; now subst
+  end;
+
+  repeat match goal with
+  (* basic inductive cases *)
+  | H1 : _ ⊩ ?e ⇝ ?e1 , H2 : _ ⊩ ?e ⇝ ?e2 |- _ =>
+      assert (e1 = e2) by auto; clear H1 H2
+  (* inductive cases with locally nameless mess *)
+  | H1 : forall x, x `notin` ?L1 → _ ⊩ _ ⇝ ?e1 ^`' x
+  , H2 : forall x, x `notin` ?L2 → _ ⊩ _ ⇝ ?e2 ^`' x
+    |- _ => pick fresh x for
+      (L1 `union` L2 `union` fv_bexpr e1 `union` fv_bexpr e2);
+         assert (e1 ^`' x = e2 ^`' x) by eauto;
+         assert (e1 = e2) by (eapply open_bexpr_wrt_bexpr_inj; eauto)
+  end;
+  congruence.
+Qed.
+
+Lemma inst_wl_split : forall Γ1' Γ2' Γ Θ Θ'
+  , Θ ⊩ Γ1' ⫢′ Γ2' ⟿ Γ ⫣ Θ'
+  → exists Γ1 Γ2 Θ0
+    , Γ = Γ1 ⫢ Γ2
+    ∧ Θ  ⊩ Γ1' ⟿ Γ1 ⫣ Θ0
+    ∧ Θ0 ⊩ Γ2' ⟿ Γ2 ⫣ Θ'.
+Proof.
+  induction Γ2'; simpl; intros.
+  - exists Γ, dwl_nil, Θ'; simpl; auto.
+  - inversion H; subst.
+    pose proof (IHΓ2' _ _ _ H3) as (Γ1 & Γ2 & Θ0 & E & Inst1 & Inst2).
+    exists Γ1, (Γ2 ⊨ w0), Θ0. repeat split; eauto.
+  - destruct b; inversion H; subst.
+    + pose proof (IHΓ2' _ _ _ H4) as (Γ1 & Γ2 & Θ0 & E & Inst1 & Inst2).
+      exists Γ1, (Γ2 ,′' x : A0), Θ0.
+      subst. repeat split; auto.
+    + pose proof (IHΓ2' _ _ _ H5) as (Γ1 & Γ2 & Θ0 & E & Inst1 & Inst2).
+      exists Γ1, Γ2, Θ0.
+      subst. repeat split; auto.
+    + pose proof (IHΓ2' _ _ _ H3) as (Γ1 & Γ2 & Θ0 & E & Inst1 & Inst2).
+      exists Γ1, Γ2, Θ0.
+      subst. repeat split; auto.
+Qed.
+
+Scheme wl_mut   := Induction for worklist Sort Prop
+  with work_mut := Induction for work     Sort Prop.
+
+Scheme winst_mut   := Induction for inst_work Sort Prop
+  with wlinst_mut := Induction for inst_wl   Sort Prop.
+
+Lemma inst_wl_ss_extend : forall Θ Γ' Γ Θ'
+  , Θ ⊩ Γ' ⟿ Γ ⫣ Θ'
+  → exists Θ0, Θ ;; Θ0 = Θ'.
+Proof.
+  intros * H.
+  pattern Θ, Γ', Γ, Θ', H.
+  apply wlinst_mut with
+    (P := fun Θ w' w Θ' (_ : Θ ⊩ w' ⇝′ w ⫣ Θ') => exists Θ0, Θ ;; Θ0 = Θ');
+    intros.
+
+  - now exists nil.
+  - now exists nil.
+  - pick fresh x. eauto.
+  - pick fresh x. eauto.
+  - pick fresh x. eauto.
+  - now exists nil.
+
+  - destruct H0. destruct H1. subst. now exists (x ;; x0).
+  - destruct H0. subst. now exists (x0; x : A !).
+  - destruct H0. subst. now exists (x0; x ≔ ⧼k⧽).
+  - destruct H0. subst. now exists (x0; x : A ≔ e).
+Qed.
+
+Lemma inst_w_ss_extend : forall Θ w' w Θ'
+  , Θ ⊩ w' ⇝′ w ⫣ Θ'
+  → exists Θ0, Θ ;; Θ0 = Θ'.
+Proof.
+  induction 1; solve
+    [now exists nil
+    | pick fresh x; eauto using inst_wl_ss_extend].
+Qed.
+
+Lemma inst_e_weakening : forall Θ1 Θ2 e' e Θ'
+  , Θ1 ;; Θ2 ⊩ e' ⇝ e → wf_ss (Θ1 ;; Θ' ;; Θ2)
+  → Θ1 ;; Θ' ;; Θ2 ⊩ e' ⇝ e.
+Proof.
+  intros * H.
+  dependent induction H; intros; eauto 4.
+Qed.
+
+#[local]
+Hint Resolve inst_e_weakening : inst_weakening.
+
+Lemma inst_ob_weakening : forall Θ1 Θ2 Θ' ob' ob,
+  Θ1 ;; Θ2 ⊩ ob' ⇝? ob → Θ1 ;; Θ' ;; Θ2 ⊩ ob' ⇝? ob.
+Proof.
+  induction 1; eauto.
+Qed.
+
+#[local]
+Hint Resolve inst_ob_weakening : inst_weakening.
+
+Lemma wf_ss_unapp : forall xs ys,
+    wf_ss (xs ;; ys) → wf_ss xs.
+Proof.
+  induction ys; intros.
+  - assumption.
+  - inversion H; auto.
+Qed.
+
+Lemma wf_ss_uncons : forall xs x,
+    wf_ss (x :: xs) → wf_ss xs.
+Proof.
+  destruct x; inversion 1; auto.
+Qed.
+
+
+Hint Immediate wf_ss_unapp wf_ss_uncons : inst_weakening.
+
+Ltac clear_app_suffix_impl :=
+  match goal with
+  | H : ?xs = ?ys ++ ?xs |- _ =>
+      assert (ys = nil) as -> by
+        now apply app_nil_invert in H
+  | H : ?ys ++ ?xs = ?xs |- _ =>
+      symmetry in H
+  | H : ?ys ++ ?xs = ?zs ++ ?xs |- _ =>
+      apply app_inj_l in H
+  | H : ?ys1 ++ ?ys2 ++ ?xs = ?zs ++ ?xs |- _ =>
+      rewrite (app_assoc ys1 ys2 xs) in H
+  | H : ?zs ++ ?xs = ?ys1 ++ ?ys2 ++ ?xs |- _ =>
+      symmetry in H
+  | H : ?x :: ?ys ++ ?xs = ?zs ++ ?xs |- _ =>
+      rewrite <- (cons_app_assoc _ x ys xs) in H;
+      clear_app_suffix_impl
+  end; simpl in *
+.
+
+Ltac clear_app_suffix :=
+  repeat progress clear_app_suffix_impl.
+
+Ltac simplify_list_eq :=
+  repeat (subst || clear_app_suffix);
+  repeat rewrite <- app_assoc in *;
+  simpl in *.
+
+Ltac conclude_ss_extend_impl :=
+  let process t1 t2 tac :=
+    let t3 := fresh "Θ" in
+    let E  := fresh "E" in
+    lazymatch t2 with
+    (* t2 is already an extension of t1 *)
+    | t1 ;; ?t => fail
+    | _ =>
+        lazymatch goal with
+        (* the equality we want to conclude already exists *)
+        | _ : t1 ;; ?t = t2 |- _ => fail
+        (* doing actual stuff *)
+        | _ => assert (exists t, t1 ;; t = t2) as [t3 E] by tac
+        end
+    end
+  in
+  match goal with
+  | H : ?t1 ⊩ _ ⟿ _ ⫣ ?t2 |- _ =>
+      process t1 t2 ltac:(eapply inst_wl_ss_extend; eassumption)
+  | H : ?t1 ⊩ _ ⇝′ _ ⫣ ?t2 |- _ =>
+      process t1 t2 ltac:(eapply inst_w_ss_extend; eassumption)
+  end
+.
+
+Ltac conclude_ss_extend :=
+  repeat conclude_ss_extend_impl.
+
+Lemma inst_wl_weakening : forall Θ1 Θ2 Θ3 Γ' Γ
+  , Θ1 ;; Θ2 ⊩ Γ' ⟿ Γ ⫣ Θ1 ;; Θ2 ;; Θ3
+  → forall Θ', wf_ss (Θ1 ;; Θ' ;; Θ2 ;; Θ3)
+  → Θ1 ;; Θ' ;; Θ2 ⊩ Γ' ⟿ Γ ⫣ Θ1 ;; Θ' ;; Θ2 ;; Θ3.
+Proof.
+  intros * H.
+  (* manual dependent mutual induction *)
+  remember (Θ1 ;; Θ2 ;; Θ3) as Θ'.
+  remember (Θ1 ;; Θ2) as Θ.
+  generalize dependent Θ3;
+  generalize dependent Θ2;
+  generalize dependent Θ1.
+  pattern Θ, Γ', Γ, Θ', H.
+  apply wlinst_mut with
+    (P := fun Θ w' w Θ0 (_ : Θ ⊩ w' ⇝′ w ⫣ Θ0) =>
+      forall Θ1 Θ2 Θ3 Θ', Θ = Θ1 ;; Θ2 → Θ0 = Θ1 ;; Θ2 ;; Θ3
+      → wf_ss (Θ1 ;; Θ' ;; Θ2 ;; Θ3)
+      → Θ1 ;; Θ' ;; Θ2 ⊩ w' ⇝′ w ⫣ Θ1 ;; Θ' ;; Θ2 ;; Θ3);
+    intros; subst.
+
+  (* inst_w *)
+  - clear_app_suffix; eauto 6 with inst_weakening.
+  - clear_app_suffix; eauto 6 with inst_weakening.
+  - eauto with inst_weakening.
+  - eauto with inst_weakening.
+  - eauto with inst_weakening.
+
+  (* inst_wl *)
+  - clear_app_suffix. auto.
+  - conclude_ss_extend. simplify_list_eq.
+    eapply instwl_cons.
+    + eauto with inst_weakening.
+    + replace (Θ1;; Θ'1;; Θ2;; Θ0;; Θ4) with
+        (Θ1;; Θ'1;; (Θ2;; Θ0);; Θ4) by
+        now repeat rewrite <- app_assoc.
+    rewrite (app_assoc Θ0 Θ2 (Θ1 ;; Θ'1)).
+    apply H1; eauto 4; rewrite <- app_assoc; auto.
+  - conclude_ss_extend; simplify_list_eq.
+    inversion H1; subst; constructor; auto.
+    + rewrite app_assoc; apply inst_e_weakening;
+      now rewrite <- app_assoc.
+  - conclude_ss_extend; simplify_list_eq.
+    inversion H1; subst. constructor; auto.
+  - conclude_ss_extend; simplify_list_eq.
+    inversion H1; subst. constructor; auto.
+    + rewrite app_assoc; apply inst_e_weakening;
+       now rewrite <- app_assoc.
+Qed.
+
+Hint Resolve inst_wl_weakening : inst_weakening.
+
+Lemma inst_w_weakening : forall Θ1 Θ2 Θ3 w' w
+  , Θ1 ;; Θ2 ⊩ w' ⇝′ w ⫣ Θ1 ;; Θ2 ;; Θ3
+  → forall Θ', wf_ss (Θ1;; Θ';; Θ2 ;; Θ3)
+  → Θ1 ;; Θ' ;; Θ2 ⊩ w' ⇝′ w ⫣ Θ1 ;; Θ' ;; Θ2 ;; Θ3.
+Proof.
+  intros * H.
+  dependent induction H; intros;
+    clear_app_suffix; eauto 6 with inst_weakening.
+Qed.
+
+Lemma bexpr_subst_open_comm : forall x v1 e v2
+  , lc_bexpr v1 → x `notin` fv_bexpr v2
+  → ([v1 /' x] e) ^^' v2 = [v1 /' x] e ^^' v2.
+Proof.
+  intros.
+  rewrite subst_bexpr_open_bexpr_wrt_bexpr.
+  rewrite (subst_bexpr_fresh_eq v2).
+  all: easy.
+Qed.
+
+Lemma aexpr_subst_open_comm : forall x v1 e v2
+  , lc_aexpr v1 → x `notin` fv_aexpr v2
+  → ([v1 /′ x] e) ^^′ v2 = [v1 /′ x] e ^^′ v2.
+Proof.
+  intros.
+  rewrite subst_aexpr_open_aexpr_wrt_aexpr.
+  rewrite (subst_aexpr_fresh_eq v2).
+  all: easy.
+Qed.
+
+
+Lemma bexpr_subst_open_var_comm : forall x1 x2 v e
+  , lc_bexpr v → x1 <> x2
+  → ([v /' x1] e) ^`' x2 = [v /' x1] e ^`' x2.
+Proof.
+  intros. rewrite bexpr_subst_open_comm; auto.
+Qed.
+
+Hint Rewrite bexpr_subst_open_comm aexpr_subst_open_comm : ln.
+Hint Extern 4 => progress autorewrite with ln : ln.
+
+Lemma notin_ss_sse : forall e x x' s,
+  x `notin` fv_ss s → binds x' e s → x `notin` fv_sse e.
+Proof.
+  induction s; intros.
+  - inversion H0.
+  - destruct H0.
+    + subst. simpl in H. auto.
+    + eapply IHs. destruct a; simpl in H. auto. auto.
+Qed.
+
+Lemma inst_e_rename : forall Θ e' e x x'
+  , Θ ⊩ e' ⇝ e → x `notin` fv_ss Θ
+  → Θ ⊩ [`′ x' /′ x] e' ⇝ [`' x' /' x] e.
+Proof.
+  intros; induction H; simpl; auto.
+  - unfold eq_dec. destruct (EqDec_eq_of_X x0 x); auto.
+  - rewrite subst_bexpr_fresh_eq.
+    + eauto.
+    + eapply notin_ss_sse with (e := sse_ex A e) in H0;
+        simpl in *; eauto.
+  - apply inste_abs  with (add x L); eauto with ln.
+  - apply inste_bind with (add x L); eauto with ln.
+  - apply inste_pi   with (add x L); eauto with ln.
+  - apply inste_all  with (add x L); eauto with ln.
+Qed.
+
+Lemma notin_open_bexpr_rec : forall x v e n
+  , x `notin` fv_bexpr v → x `notin` fv_bexpr e
+  → x `notin` fv_bexpr (open_bexpr_wrt_bexpr_rec n v e).
+Proof.
+  induction e; simpl; intros; auto.
+  - destruct (lt_eq_lt_dec n n0); auto.
+    destruct s; auto.
+Qed.
+
+Lemma notin_open_bexpr : forall x v e
+  , x `notin` fv_bexpr v → x `notin` fv_bexpr e
+  → x `notin` fv_bexpr (e ^^' v).
+Proof.
+  intros. now eapply notin_open_bexpr_rec.
+Qed.
+
+Lemma notin_close_bexpr_rec : forall x e n,
+    x `notin` fv_bexpr (close_bexpr_wrt_bexpr_rec n x e).
+Proof.
+  induction e; simpl; intros; auto.
+  - destruct (lt_ge_dec n n0); auto.
+  - unfold eq_dec. destruct EqDec_eq_of_X; auto.
+Qed.
+
+Lemma notin_close_bexpr : forall x e,
+    x `notin` fv_bexpr (close_bexpr_wrt_bexpr x e).
+Proof.
+  intros. apply notin_close_bexpr_rec.
+Qed.
+
+Hint Resolve notin_close_bexpr : atoms.
+Hint Resolve notin_open_bexpr : atoms.
+
+Hint Resolve inst_ae_lc : lc.
+Hint Resolve inst_e_lc : lc.
+
+Hint Rewrite close_bexpr_wrt_bexpr_open_bexpr_wrt_bexpr : ln.
+Hint Rewrite <- subst_bexpr_close_bexpr_wrt_bexpr : ln.
+Hint Rewrite open_bexpr_wrt_bexpr_close_bexpr_wrt_bexpr : ln.
+
+Ltac rev_subst_gather_atoms :=
+  let L0 := gather_atoms_with (fun x : atom => {{ x }}) in
+  let L1 := gather_atoms_with (fun x : atoms => x) in
+  let L2 := gather_atoms_with (fun x : bexpr => fv_bexpr x) in
+  let L3 := gather_atoms_with (fun x : aexpr => fv_aexpr x) in
+  let L4 := gather_atoms_with (fun x : subst_set => fv_ss x) in
+  constr:(L0 `union` L1 `union` L2 `union` L3 `union` L4).
+
+Tactic Notation "pick" "fresh" ident(x) "for" "all" :=
+  let L  := rev_subst_gather_atoms in
+  pick fresh x for L.
+
+Ltac e_rev_subst_apply_ih :=
+  match goal with
+  | IH : forall _ _ _, _ → _ ⊩ [?v /′ ?x] ?e ^`′ _ ⇝ _ → _
+  , H  : _ ⊩ ([?v /′ ?x] ?e) ^`′ _ ⇝ ?e1 ^`' _ |- _ =>
+    let e1' := fresh e1 in
+    let E := fresh "E" in
+    let H' := fresh "H" in
+    rewrite aexpr_subst_open_comm in H; eauto 3 with lc;
+    apply IH in H as (e1' & E & H'); auto with atoms
+  | IH : forall _ _, _ → _ ⊩ [?v /′ ?x] ?e ⇝ _ → _
+  , H  : _ ⊩ [?v /′ ?x] ?e ⇝ ?e1 |- _ =>
+    let e1' := fresh e1 in
+    let E := fresh "E" in
+    let H' := fresh "H" in
+    apply IH in H as (e1' & E & H'); auto with atoms
+  end
+.
+
+Ltac inst_cofinite_impl H x :=
+  match type of H with
+  | forall x, x `notin` ?L -> _ =>
+      let Fr := fresh "Fr" in
+      assert (x `notin` L) as Fr by auto;
+      specialize (H x Fr); clear Fr
+  end
+.
+
+Ltac inst_cofinites_with x :=
+  repeat
+    match goal with
+    | H : forall x0, x0 `notin` ?L → _ |- _ =>
+      inst_cofinite_impl H x
+    end
+.
+
+Ltac inst_cofinites :=
+  match goal with
+  | x : atom |- _ => inst_cofinites_with x
+  end.
+
+Ltac inst_cofinites_with_new :=
+  let x := fresh "x" in
+  pick fresh x; inst_cofinites_with x.
+
+Ltac inst_cofinites_by F :=
+  let L := F in
+  let x := fresh "x" in
+  pick fresh x for L; inst_cofinites_with x.
+
+
+Lemma bexpr_open_r_close_l : forall e1 e2 x,
+    x `notin` fv_bexpr e2 → e1 = e2 ^`' x → e1 \`' x = e2.
+Proof.
+  intros * Fr H.
+  assert (e1 \`' x = e2 ^`' x \`' x) by now rewrite H.
+  now rewrite close_bexpr_wrt_bexpr_open_bexpr_wrt_bexpr in H0.
+Qed.
+
+Ltac pick_different x :=
+  match goal with
+  | x2 : atom |- _ =>
+      lazymatch x2 with
+      | x => fail
+      | _ => constr:(x2)
+      end
+  end.
+
+Ltac prepare_rename_impl :=
+  match goal with
+  | |- context [?e ^`' ?x] =>
+      lazymatch goal with
+      (* don't rename if it's wrapped inside other open or subst *)
+      | |- context [e ^`' x ^`' ?x'] => fail
+      | |- context [[`' ?x' /' x] e ^`' x] => fail
+      | _ => let x1 := pick_different x in
+            rewrite (subst_bexpr_intro x1)
+      end
+  | |- context [?e ^`′ ?x] =>
+      lazymatch goal with
+      | |- context [e ^`′ x ^`′ ?x'] => fail
+      | |- context [[`′ ?x' /′ x] e ^`′ x] => fail
+      | _ => let x1 := pick_different x in
+            rewrite (subst_aexpr_intro x1)
+      end
+  end; auto 2 with atoms
+.
+
+Ltac prepare_rename := repeat prepare_rename_impl.
+
+Lemma inst_e_rev_subst : forall v' v x e'
+  , lc_aexpr e' → forall e0 Θ, x `notin` fv_bexpr e0
+  → Θ ⊩ [v' /′ x] e' ⇝ e0 → Θ ⊩ v' ⇝ v
+  → exists e, [v /' x] e = e0 ∧ Θ ⊩ e' ⇝ e.
+Proof.
+  intros * Lc.
+  induction Lc; simpl; intros * Fr He Hv;
+    lazymatch type of He with
+      (* only if it's a variable it doesn't invert the hypo *)
+    | _ ⊩ (if _ then _ else _) ⇝ _ => idtac
+    | _ ⊩ ⧼ ?k ⧽′ ⇝ _ => destruct k; inversion He; subst
+    | _ => inversion He; subst; simpl in Fr;
+          (* instantiate cofinite for those with binders *)
+          inst_cofinites_by rev_subst_gather_atoms;
+          repeat e_rev_subst_apply_ih
+    end.
+  - exists (`' x0). simpl.
+    unfold eq_dec in *. destruct (EqDec_eq_of_X x0 x).
+    + assert (v = e0) by (eapply inst_e_det with (Θ := Θ); eauto).
+      eauto.
+    + inversion He. now subst.
+  - exists ⋆'; eauto.
+  - exists ◻'; eauto.
+  - exists ⧼ k ⧽'; eauto.
+  - exists e0. eauto with lngen.
+  - exists (be_num n); eauto.
+  - exists be_int; eauto.
+  - exists be_bot; eauto.
+  - exists (be_app f0 a0); subst; auto.
+  - exists (be_abs (e0 \`' x0)). split.
+    + simpl. f_equal.
+      rewrite subst_bexpr_close_bexpr_wrt_bexpr; eauto with lc.
+      apply bexpr_open_r_close_l; auto.
+    + apply inste_abs with L; intros.
+      prepare_rename.
+      apply inst_e_rename; autorewrite with ln; auto.
+  - exists (be_pi A1 (B1 \`' x0)). split.
+    + simpl. f_equal. assumption.
+      rewrite subst_bexpr_close_bexpr_wrt_bexpr; eauto with lc.
+      apply bexpr_open_r_close_l; auto.
+    + apply inste_pi with L; intros; auto.
+      prepare_rename; apply inst_e_rename;
+        autorewrite with ln; auto.
+  - exists (be_bind (e0 \`' x0)). split.
+    + simpl. f_equal.
+      rewrite subst_bexpr_close_bexpr_wrt_bexpr; eauto with lc.
+      apply bexpr_open_r_close_l; auto.
+    + apply inste_bind with L; intros; auto.
+      prepare_rename. apply inst_e_rename; autorewrite with ln; auto.
+  - exists (be_all A1 (B1 \`' x0)). split.
+    + simpl. f_equal. assumption.
+      rewrite subst_bexpr_close_bexpr_wrt_bexpr; eauto with lc.
+      apply bexpr_open_r_close_l; auto.
+    + apply inste_all with L; intros; auto.
+      prepare_rename; apply inst_e_rename;
+        autorewrite with ln; auto.
+  - exists (be_castup e0); subst; auto.
+  - exists (be_castdn e0); subst; auto.
+  - exists (e0 ::' A1); subst; auto.
+Qed.
+
+Scheme wl_lc_mut := Induction for lc_worklist Sort Prop
+  with  w_lc_mut := Induction for lc_work Sort Prop.
+
+Lemma inst_wl_rev_subst : forall Γ' x e' e
+  , lc_worklist Γ' → forall Γ0 Θ Θ', x `notin` fv_dworklist Γ0
+  → Θ ⊩ subst_worklist e' x Γ' ⟿ Γ0 ⫣ Θ'
+  → Θ ⊩ e' ⇝ e
+  → exists Γ
+    , subst_dworklist e x Γ = Γ0
+    ∧ Θ ⊩ Γ' ⟿ Γ ⫣ Θ'.
+Proof.
+  intros * H.
+  pattern Γ', H.
+  apply wl_lc_mut with
+    (P0 := fun w' (_ : lc_work w') =>
+      forall x w0 Θ Θ'
+      , x `notin` fv_dwork w0
+      → Θ ⊩ subst_work e' x w' ⇝′ w0 ⫣ Θ'
+      → Θ ⊩ e' ⇝ e
+      → exists w, subst_dwork e x w = w0 ∧ Θ ⊩ w' ⇝′ w ⫣ Θ'); simpl; intros.
+  - inversion H1; subst. exists dwl_nil; simpl; split; auto.
+  - inversion H3; subst. simpl in H2.
+    apply H0 in H8; auto. apply H1 in H11; auto.
+(*
+  simpl; intros.
+  - inversion H; subst.
+    exists dwl_nil; simpl; repeat split; auto.
+  - simpl in H1. inversion H1; subst. admit.
+  - destruct b; inversion H0; subst; simpl in *; admit.
+  - admit.
+  -
+*)
+Admitted.
